Reflection/Derive.lean
@@ -3,8 +3,9 @@ import Reflection.MutualInductive
 import Qq
 
 open Lean Meta Elab Term Qq
+open Reflection MutualInductive
 
-#check InductiveVal
+namespace Reflection.MutualInductive.Derive
 
 private partial def getTyₛ (tys : Expr) : MetaM Q(Tyₛ.{u}) := do
   forallBoundedTelescope tys (some 1) fun var body => do
@@ -17,53 +18,85 @@ private partial def getTyₛ (tys : Expr) : MetaM Q(Tyₛ.{u}) := do
       let rest : Q($ty -> Tyₛ.{u}) <- mkLambdaFVars #[var] rest
       return q(Tyₛ.SPi.{u} $ty $rest)
 
--- def skipParams (nParams : Nat) (e : Expr) : MetaM Expr := do
---   forallBoundedTelescope
+partial def skipParams (tys : Expr) (nParams : Nat) (cont : Expr -> MetaM Expr) : MetaM Expr :=
+  match nParams with
+  | 0 => cont tys
+  | nParams + 1 => do
+    forallBoundedTelescope tys (some 1) fun var body => do
+      let body' <- skipParams body nParams cont
+      if body'.containsFVar var[0]!.fvarId! then mkLambdaFVars var body'
+      else return body'
 
-elab "%Tyₛ " t:term : term => do
-  let t <- elabTermAndSynthesize t none
+elab "Tyₛ% " tys:term : term => do
+  let tys <- elabTerm tys none
   let u <- mkFreshLevelMVar
-  getTyₛ (u:=u) t
--- elab "%Tyₛ " i:ident : term => do
---   let ind <- getConstInfoInduct i.getId
---   let u <- mkFreshLevelMVar
---   getTyₛ (u:=u) ind.type
+  getTyₛ (u:=u) tys
 
-#check Nat
-
-#check %Tyₛ (Nat -> Type)
-
-/-- Given a `T` such as `Vec 123 : Type`, produce `Tmₛ.app (Tmₛ.var Varₛ.vz) 123 : Tmₛ _ Tyₛ.U`.
-  Given `Vec : Nat -> Type`, produce `Tmₛ.var Varₛ.vz : Tmₛ _ (Tyₛ.SPi Nat fun _ => Tyₛ.U)`. -/
-private partial def getTmₛ (Γₛ : Q(Conₛ.{u})) (Aₛ : Q(Tyₛ.{u})) (T : Expr) : MetaM Q(Tmₛ.{u} $Γₛ $Aₛ) := do
-  match <- Meta.whnf T with
-  | .app t u =>
-    let t := t
-    let tt <- getTmₛ Γₛ Aₛ t
-    q(Tmₛ.app )
-  | .fvar _ => q(Tmₛ.var Varₛ.vz)
-  | _ => throwError "uh oh"
-
-elab "%Tmₛ " T:term : term => do
+elab "Tyₛ! " T:term : term => do
   let T <- elabTerm T none
-  -- let  := T.getAppFn
-  let ind <- getConstInfoInduct (getAppFn)
-  getTyₚ ind.type
+  let ⟨I, args⟩ := T.getAppFnArgs
+  let info <- getConstInfoInduct I
+  if info.numParams != args.size then throwError m!"Expected {info.numParams} params."
+  let u <- mkFreshLevelMVar
+  skipParams info.type info.numParams (getTyₛ (u := u))
 
-private partial def getTyₚ (Γₛ : Q(Conₛ.{u})) (args : Expr) : MetaM Q(Tyₚ.{u} $Γₛ) := do
-  forallBoundedTelescope args (some 1) fun var body => do
+elab "Conₛ! " T:term : term => do
+  let T <- elabTerm T none
+  let ⟨I, args⟩ := T.getAppFnArgs
+  let info <- getConstInfoInduct I
+  if info.numParams != args.size then throwError m!"Expected {info.numParams} params."
+  let u <- mkFreshLevelMVar
+  info.all.foldlM (fun (acc : Q(Conₛ.{u})) name => do
+    let info <- getConstInfoInduct name
     let u <- mkFreshLevelMVar
+    let ty : Q(Tyₛ.{u}) <- skipParams info.type info.numParams (getTyₛ (u := u))
+    return q(Conₛ.ext $acc $ty)
+  ) q(Conₛ.nil.{u})
+
+#check Tyₛ% (Nat -> Type)
+#check Tyₛ! (Vec String)
+#check Conₛ! (Vec String)
+
+-- /-- Given a `T` such as `Vec 123 : Type`, produce `Tmₛ.app (Tmₛ.var Varₛ.vz) 123 : Tmₛ _ Tyₛ.U`.
+--   Given `Vec : Nat -> Type`, produce `Tmₛ.var Varₛ.vz : Tmₛ _ (Tyₛ.SPi Nat fun _ => Tyₛ.U)`. -/
+-- private partial def getTmₛ (Γₛ : Q(Conₛ.{u})) (Aₛ : Q(Tyₛ.{u})) (T : Expr) : MetaM Q(Tmₛ.{u} $Γₛ $Aₛ) := do
+--   match <- Meta.whnf T with
+--   | .app t u =>
+--     let t := t
+--     let tt <- getTmₛ Γₛ Aₛ t
+--     sorry
+--     -- q(Tmₛ.app )
+--   | .fvar _ => q(Tmₛ.var Varₛ.vz)
+--   | _ => throwError "uh oh"
+
+-- elab "%Tmₛ " T:term : term => do
+--   let T <- elabTerm T none
+--   -- let  := T.getAppFn
+--   let ind <- getConstInfoInduct (getAppFn)
+--   getTyₚ ind.type
+
+partial def getTyₚ (Γₛ : Q(Conₛ.{u})) (tys : Expr) : MetaM Q(Tyₚ.{u} $Γₛ) := do
+  forallBoundedTelescope tys (some 1) fun var body => do
     if var.isEmpty then
-      -- body is e.g. `Vec 123`.
-      let T <- getTmₛ Γₛ q(Tyₛ.U) body
-      return q(Tyₚ.El $(T))
+      return q(Tyₛ.U.{u})
     else
       let var := var[0]!
       let ty : Q(Type u) <- var.fvarId!.getType
-      let rest : Expr <- getTyₛ body -- rest is for example `var : X ⊢ SPi ...`
-      let rest : Q($ty -> Tyₛ.{u}) <- mkLambdaFVars #[var] rest -- rest is for example `⊢ fun var:X => SPi ...`
+      let rest : Q(Tyₛ.{u}) <- getTyₛ body -- rest is for example `var : X ⊢ SPi ...`
+      let rest : Q($ty -> Tyₛ.{u}) <- mkLambdaFVars #[var] rest
       return q(Tyₛ.SPi.{u} $ty $rest)
-
+  -- forallBoundedTelescope args (some 1) fun var body => do
+  --   let u <- mkFreshLevelMVar
+  --   if var.isEmpty then
+  --     -- body is e.g. `Vec 123`.
+  --     let T <- getTmₛ Γₛ q(Tyₛ.U) body
+  --     return q(Tyₚ.El $(T))
+  --   else
+  --     let var := var[0]!
+  --     let ty : Q(Type u) <- var.fvarId!.getType
+  --     let rest : Expr <- getTyₛ body -- rest is for example `var : X ⊢ SPi ...`
+  --     let rest : Q($ty -> Tyₛ.{u}) <- mkLambdaFVars #[var] rest -- rest is for example `⊢ fun var:X => SPi ...`
+  --     return q(Tyₛ.SPi.{u} $ty $rest)
 
 elab "%Tyₚ " i:ident : term => do
   let ind <- getConstInfoInduct i.getId
